theories/Util.v
@@ -7,6 +7,18 @@ Require Import Coq.Classes.DecidableClass.
 Require Import Coq.Lists.List.
 Require Import Coq.Strings.String.
 
+Definition resolve (t : Type) : Type := t.
+Definition use {t} (r : resolve t) : t := r.
+Existing Class resolve.
+Typeclasses Transparent resolve.
+Hint Extern 1 (resolve _) => red : typeclass_instances.
+
+Lemma decide_ok : forall P {ok : Decidable P}, decide P = true <-> P.
+Proof.
+  intros. eapply Decidable_spec.
+Qed.
+
+
 (* note(gmm): this file should be eliminated in favor of definitions defined elsewhere, e.g. in ExtLib *)
 
 Section find_in_list.
@@ -28,8 +40,14 @@ Global Instance Decidable_eq_string (a b : string) : Decidable (a = b) :=
   {| Decidable_witness := String.eqb a b
    ; Decidable_spec := @String.eqb_eq a b |}.
 
+Global Instance Decidable_eq_ascii (a b : Ascii.ascii) : Decidable (a = b) :=
+  {| Decidable_witness := Ascii.eqb a b
+   ; Decidable_spec := @Ascii.eqb_eq a b |}.
+
 Section dec_list.
-  Context {T : Type} {dec : forall a b : T, Decidable (a = b)}.
+  Context {T : Type} {dec : resolve (forall a b : T, Decidable (a = b))}.
+  Let dec' := use dec.
+  Existing Instance dec'.
 
   Fixpoint dec_list (a b : list T) : bool :=
     match a , b with
@@ -42,15 +60,9 @@ Section dec_list.
     forall a b : list T, dec_list a b = true <-> a = b.
   Proof.
     induction a; destruct b; simpl; intros; try solve [ tauto | split; congruence ].
-    split.
-    - intros. eapply Bool.andb_true_iff in H. destruct H.
-      eapply Decidable_sound in H.
-      eapply IHa in H0. f_equal; assumption.
-    - inversion 1; subst.
-      eapply Bool.andb_true_iff.
-      split.
-      eapply Decidable_complete. auto.
-      eapply IHa. reflexivity.
+    rewrite Bool.andb_true_iff.
+    rewrite decide_ok. rewrite IHa.
+    firstorder (try congruence).
   Qed.
 
   Global Instance Decidable_eq_list (a b : list T) : Decidable (a = b) :=
@@ -67,10 +79,8 @@ Section dec_list.
   Lemma dec_option_ok : forall a b, dec_option a b = true <-> a = b.
   Proof.
     destruct a; destruct b; simpl; try solve [ tauto | split; congruence ].
-    generalize (dec t t0).
-    destruct d.
-    simpl. etransitivity. eassumption.
-    split; congruence.
+    rewrite decide_ok.
+    firstorder congruence.
   Qed.
 
   Global Instance Decidable_eq_option (a b : option T) : Decidable (a = b) :=
@@ -81,8 +91,12 @@ End dec_list.
 
 Section dec_sum.
   Context {T U : Type}
-          {decT : forall a b : T, Decidable (a = b)}
-          {decU : forall a b : U, Decidable (a = b)}.
+          {decT : resolve (forall a b : T, Decidable (a = b))}
+          {decU : resolve (forall a b : U, Decidable (a = b))}.
+  Let decT' := use decT.
+  Let decU' := use decU.
+  Existing Instance decT'.
+  Existing Instance decU'.
 
   Definition dec_sum (a b : T + U) : bool :=
     match a , b with
@@ -118,3 +132,23 @@ Section dec_sum.
    ; Decidable_spec := dec_prod_ok a b |}.
 
 End dec_sum.
+
+Definition Decidable_dec {T} (a b : T) {Dec : Decidable (a = b)}
+  : {a = b} + {a <> b}.
+Proof.
+  destruct Dec.
+  destruct Decidable_witness.
+  - left. apply Decidable_spec. reflexivity.
+  - right. intro. apply Decidable_spec in H. congruence.
+Defined.
+
+(* note(gmm): this isn't the most computationally efficient way to
+ * define a [Decidable] instance, but it is convenient because
+ * of [decide equality].
+ *)
+Definition dec_Decidable {T} {a b : T} (Dec : {a = b} + {a <> b})
+  : Decidable (a = b).
+Proof.
+  refine {| Decidable_witness := if Dec then true else false |}.
+  destruct Dec; split; congruence.
+Defined.
